Main.lean
@@ -1,4 +1,72 @@
-import «Lean4Repl»
+import Lean4Repl
 
-def main : IO Unit :=
-  IO.println s!"Hello, {hello}!"
+import Mathlib.Data.Nat.Factors
+import Mathlib.Data.Nat.Prime
+import Mathlib.Tactic.NormNum.Basic
+
+#align_import data.nat.prime_norm_num from "leanprover-community/mathlib"@"10b4e499f43088dd3bb7b5796184ad5216648ab1"
+
+/-!
+Contains an example MWE file for the Lean 4 Repl.
+This file's content will be replaced by the MWE
+of the user to execute the lean4repl.
+-/
+
+
+/-!
+# `norm_num` extensions on natural numbers
+
+This file provides a `norm_num` extension to prove that natural numbers are prime and compute
+its minimal factor. Todo: compute the list of all factors.
+
+
+## Implementation Notes
+
+For numbers larger than 25 bits, the primality proof produced by `norm_num` is an expression
+that is thousands of levels deep, and the Lean kernel seems to raise a stack overflow when
+type-checking that proof. If we want an implementation that works for larger primes, we should
+generate a proof that has a smaller depth.
+
+Note: `evalMinFac.aux` does not raise a stack overflow, which can be checked by replacing the
+`prf'` in the recursive call by something like `(.sort .zero)`
+-/
+
+open Nat Qq Lean Meta
+
+namespace Mathlib.Meta.NormNum
+
+theorem not_prime_mul_of_ble (a b n : ℕ) (h : a * b = n) (h₁ : a.ble 1 = false)
+    (h₂ : b.ble 1 = false) : ¬ n.Prime :=
+  not_prime_mul' h (ble_eq_false.mp h₁) (ble_eq_false.mp h₂)
+
+/-- Produce a proof that `n` is not prime from a factor `1 < d < n`. `en` should be the expression
+  that is the natural number literal `n`. -/
+def deriveNotPrime (n d : ℕ) (en : Q(ℕ)) : Q(¬ Nat.Prime $en) := Id.run <| do
+  let d' : ℕ := n / d
+  let prf : Q($d * $d' = $en) := (q(Eq.refl $en) : Expr)
+  let r : Q(Nat.ble $d 1 = false) := (q(Eq.refl false) : Expr)
+  let r' : Q(Nat.ble $d' 1 = false) := (q(Eq.refl false) : Expr)
+  return q(not_prime_mul_of_ble _ _ _ $prf $r $r')
+
+/-- A predicate representing partial progress in a proof of `minFac`. -/
+def MinFacHelper (n k : ℕ) : Prop :=
+  2 < k ∧ k % 2 = 1 ∧ k ≤ minFac n
+
+theorem MinFacHelper.one_lt {n k : ℕ} (h : MinFacHelper n k) : 1 < n := by
+  have : 2 < minFac n := h.1.trans_le h.2.2
+  rcases eq_zero_or_pos n with rfl|h
+  · contradiction
+  rcases (succ_le_of_lt h).eq_or_lt with rfl|h
+  · contradiction
+  exact h
+
+theorem minFacHelper_0 (n : ℕ)
+    (h1 : Nat.ble (nat_lit 2) n = true) (h2 : nat_lit 1 = n % (nat_lit 2)) :
+    MinFacHelper n (nat_lit 3) := by
+    lean_dojo_repl
+    sorry
+  -- refine ⟨by norm_num, by norm_num, ?_⟩
+  -- refine (le_minFac'.mpr λ p hp hpn ↦ ?_).resolve_left (Nat.ne_of_gt (Nat.le_of_ble_eq_true h1))
+  -- rcases hp.eq_or_lt with rfl|h
+  -- · simp [(Nat.dvd_iff_mod_eq_zero ..).1 hpn] at h2
+  -- · exact h
