lakefile.lean
@@ -5,6 +5,19 @@ package «Lean4Repl» {
   -- add package configuration options here
 }
 
+lean_exe «BuildAllDependencies» {
+  root := `BuildAllDependencies
+  -- add package configuration options here
+}
+
 lean_lib «Lean4Repl» {
   -- add library configuration options here
 }
+
+@[default_target]
+lean_exe «lean4-example» {
+  root := `Main
+}
+
+require mathlib from git
+  "https://github.com/leanprover-community/mathlib4.git"@"355541ae7a2455222f179dcf7f074aa2c45eb8aa"
