README.md
@@ -1,4 +1,4 @@
-## Lean library for repl enviorment.
+## Repl env for interactive theorem testing
 
 This repo contains the Lean4Repl.lean file that helps executing lean commands against a state.
 
@@ -7,4 +7,33 @@ The builds for Lean4Repl can be built by running:
 lake build Lean4Repl
 ```
 
-and then the binaries are found in the build directory.
+### Setup:
+The to be tested theorem can be put into a environment to load the dependent packages by providing a [MWE](https://leanprover-community.github.io/mwe.html) in the MAIN.lean file. This enables loading the correct name spaces and providing definitions that can be used during the interactions.
+
+An example MWE for the theorem minFacHelper_0 is provided in the Main.lean file.
+
+To have all dependencies already build before interacting - this will save time - one can build the whole dependency of mathlib by running
+```
+lake build BuildAllDependencies
+```
+
+This creates the binaries which can then be found in the build directory and will be used to speed up all future imports
+
+
+### Running Repl:
+Simply modify the Main.lean with your setup + theorem and remove the proof by replacing it with run:
+```
+=: by lean_dojo_repl sorry
+```
+and then run
+```
+lake env lean Main.lean
+```
+and it will return:
+```
+REPL> {"tacticState": "n : ℕ\nh1 : ble 2 n = true\nh2 : 1 = n % 2\n⊢ MinFacHelper n 3", "sid": 0, "error": null}
+```
+Now, you can provide commands like this:
+```
+{"sid": 0, "cmd": [" refine \u27e8by norm_num, by norm_num, ?_\u27e9 ","  refine (le_minFac'.mpr \u03bb p hp hpn \u21a6 ?_).resolve_left (Nat.ne_of_gt (Nat.le_of_ble_eq_true h1))"," rcases hp.eq_or_lt with rfl|h"," \u00b7 simp [(Nat.dvd_iff_mod_eq_zero ..).1 hpn] at h2 "," \u00b7 exact h"]}
+```
